Introduction of LLBC#.
Subsequently, proof of simulation with LLBC+.

src/LLBC_sharp_semantics.v
@@ -188,13 +188,13 @@ Inductive LLBC_plus_eval_stmt : nat -> statement -> LLBC_sharp_state -> branchin
       S0 |-{stmt} stmt ~>{1 + n} B2
   (* We perform a single loop iteration, and stop because it does not continue. *)
   | LLBC_plus_E_Loop_Stop n S body B1
-      (eval_body : S |-{stmt} body ~>{n} B1)
+      (eval_body : S |-{stmt} body ~>{1 + n} B1)
       (* An iteration that yields `rUnit` gets stuck. *)
       (no_unit : lookup rUnit B1 = None)
       (no_continue : lookup rContinue B1 = None) :
       S |-{stmt} (LOOP {{ body }}) ~>{1 + n} (end_loop B1)
   | LLBC_plus_E_Loop_Continue n S body B1 S1 B2 Bend
-      (eval_body : S |-{stmt} body ~>{n} B1)
+      (eval_body : S |-{stmt} body ~>{1 + n} B1)
       (* An iteration that yields `rUnit` gets stuck. *)
       (no_unit : lookup rUnit B1 = None)
       (Hcontinue : lookup rContinue B1 = Some S1)
@@ -202,3 +202,64 @@ Inductive LLBC_plus_eval_stmt : nat -> statement -> LLBC_sharp_state -> branchin
       (His_join : is_join (end_loop (delete rContinue B1)) B2 Bend) :
       S |-{stmt} (LOOP {{ body }}) ~>{1 + n} Bend
 where "S |-{stmt} stmt ~>{ n } B" := (LLBC_plus_eval_stmt n stmt S B) : llbc_sharp_scope.
+
+Global Reserved Notation "S  |-#  stmt  ~>  B" (at level 50).
+
+Inductive LLBC_sharp_eval_stmt : statement -> LLBC_sharp_state -> branching_state -> Prop :=
+  | LLBC_sharp_E_Nop S : S |-# Nop ~> {[rUnit := S]}
+  | LLBC_sharp_E_Seq_Propagate S0 B1 stmt_0 stmt_1
+      (eval_stmt_0 : S0 |-# stmt_0 ~> B1) (Hno_unit : lookup rUnit B1 = None) :
+      S0 |-# (Seq stmt_0 stmt_1) ~> B1
+  | LLBC_sharp_E_Seq_Unit_Propagate S0 B1 S1 B2 stmt_0 stmt_1
+      (eval_stmt_0 : S0 |-# stmt_0 ~> B1)
+      (H_unit : lookup rUnit B1 = Some S1)
+      (leq_B1_B2 : leq_branching (delete rUnit B1) B2)
+      (eval_stmt_1 : S1 |-# stmt_1 ~> B2) :
+      S0 |-# (Seq stmt_0 stmt_1) ~> B2
+  | LLBC_sharp_E_Assign S vS' S'' p rv (eval_rv : S |-{rv} rv => vS') (Hstore : store p vS' S'') :
+      S |-# ASSIGN p <- rv ~> {[rUnit := S'']}
+  | LLBC_sharp_E_IfThenElse_T S S' B_if cond stmt_if stmt_else
+      (eval_cond : S |-{op} cond => (LLBC_sharp_bool true, S'))
+      (Heval_if_branch : S' |-# stmt_if ~> B_if) :
+      S |-# (IF cond {{ stmt_if }} ELSE {{ stmt_else }}) ~> B_if
+  | LLBC_sharp_E_IfThenElse_F S S' B_else cond stmt_if stmt_else
+      (eval_cond : S |-{op} cond => (LLBC_sharp_bool false, S'))
+      (Heval_else_branch : S' |-# stmt_else ~> B_else) :
+      S |-# (IF cond {{ stmt_if }} ELSE {{ stmt_else }}) ~> B_else
+  (* Note: in the ICFP'24 article, the symbolic value is replaced by a concrete boolean in each
+     branch. We cannot do that as symbolic values are currently not named. *)
+  | LLBC_sharp_IfThenElse_Symbolic S S' B cond stmt_if stmt_else
+      (eval_cond : S |-{op} cond => (LLBC_sharp_symbolic boolT, S'))
+      (Heval_if_branch : S' |-# stmt_if ~> B)
+      (Heval_else_branch : S' |-# stmt_else ~> B) :
+      S |-# (IF cond {{ stmt_if }} ELSE {{ stmt_else }}) ~> B
+  | LLBC_sharp_E_Reorg S0 S1 B2 stmt (Hreorg : reorg^* S0 S1) (Heval : S1 |-# stmt ~> B2) :
+      S0 |-# stmt ~> B2
+  (* We perform a single loop iteration, and stop because it does not continue. *)
+  | LLBC_sharp_E_Loop_Stop S body B1
+      (eval_body : S |-# body ~> B1)
+      (* An iteration that yields `rUnit` gets stuck. *)
+      (no_unit : lookup rUnit B1 = None)
+      (no_continue : lookup rContinue B1 = None) :
+      S |-# (LOOP {{ body }}) ~> (end_loop B1)
+  | LLBC_sharp_E_Loop_Continue S0 body B1 S1 Bend
+      (eval_body : S0 |-# body ~> B1)
+      (* An iteration that yields `rUnit` gets stuck. *)
+      (no_unit : lookup rUnit B1 = None)
+      (leq_B1_Bend : leq_branching (end_loop (delete rContinue B1)) Bend)
+      (Hcontinue : lookup rContinue B1 = Some S1)
+      (Heval2 : S1 |-# (LOOP {{ body }}) ~> Bend) :
+       S0 |-# (LOOP {{ body }}) ~> Bend
+  (* These are LLBC## only rules. *)
+  | LLBC_sharp_E_Loop_Invariant body Sinv Binv
+      (eval_body : Sinv |-# body ~> Binv)
+      (inv_preservation : lookup rContinue Binv = Some Sinv)
+      (no_unit : lookup rUnit Binv = None) :
+      Sinv |-# (LOOP {{ body }}) ~> (end_loop (delete rContinue Binv))
+  | LLBC_sharp_Weaken_Precondition s Sl Sr B
+      (Hweaken : leq_symbolic Sl Sr) (Heval : Sr |-# s ~> B) :
+      Sl |-# s ~> B
+  | LLBC_sharp_Weaken_Postcondition s S Bl Br
+      (Heval : S |-# s ~> Bl) (Hweaken : leq_branching Bl Br) :
+      S |-# s ~> Br
+where "S |-# stmt ~> B" := (LLBC_sharp_eval_stmt stmt S B) : llbc_sharp_scope.
